wip making WeakestPrecondition.cmd an alias of Semantics.exec

bedrock2/src/bedrock2/WeakestPrecondition.v
@@ -1,4 +1,5 @@
 Require Import coqutil.Macros.subst coqutil.Macros.unique coqutil.Map.Interface coqutil.Map.OfListWord.
+Require Import coqutil.Tactics.fwd.
 Require Import Coq.ZArith.BinIntDef coqutil.Word.Interface coqutil.Word.Bitwidth.
 Require Import coqutil.dlet bedrock2.Syntax bedrock2.Semantics.
 
@@ -41,6 +42,27 @@ Section WeakestPrecondition.
     Fixpoint expr e := expr_body expr e.
   End WithMemAndLocals.
 
+  Ltac t :=
+    repeat match goal with
+      | |- forall _, _ => progress intros
+      | H: exists _, _ |- _ => destruct H
+      | H: and _ _ |- _ => destruct H
+      | H: eq _ ?y |- _ => subst y
+      | _ => progress cbn in *
+      end; eauto.
+
+  Lemma expr_sound: forall m l e post (H : expr m l e post),
+    exists v, Semantics.eval_expr m l e = Some v /\ post v.
+  Proof.
+    induction e; t.
+    { eapply IHe in H; t. cbv [load] in H0; t. rewrite H. rewrite H0. eauto. }
+    { eapply IHe in H; t. cbv [load] in H0; t. rewrite H. rewrite H0. eauto. }
+    { eapply IHe1 in H; t. eapply IHe2 in H0; t. rewrite H, H0; eauto. }
+    { eapply IHe1 in H; t. rewrite H. Tactics.destruct_one_match.
+      { eapply IHe3 in H0; t. }
+      { eapply IHe2 in H0; t. } }
+  Qed.
+
   Section WithF.
     Context {A B} (f: A -> (B -> Prop) -> Prop).
     Definition list_map_body rec (xs : list A) (post : list B -> Prop) : Prop :=
@@ -54,83 +76,163 @@ Section WeakestPrecondition.
     Fixpoint list_map xs := list_map_body list_map xs.
   End WithF.
 
-  Section WithFunctions.
+  Lemma exprs_sound : forall m l args P,
+      list_map (expr m l) args P ->
+      exists x, Semantics.eval_call_args m l args = Some x /\ P x.
+  Proof.
+    induction args; cbn; repeat (subst; t).
+    eapply expr_sound in H; t; rewrite H.
+    eapply IHargs in H0; t; rewrite H0.
+    eauto.
+  Qed.
+
+  Lemma getmany_sound: forall a l P,
+      list_map (get l) a P -> exists vs, map.getmany_of_list l a = Some vs /\ P vs.
+  Proof.
+    cbv [map.getmany_of_list].
+    induction a; cbn; repeat (subst; t).
+    cbv [get] in H; t.
+    epose proof (IHa _ _ H0); clear IHa; t.
+    rewrite H. erewrite H1. eexists; split; eauto.
+  Qed.
+
+  Definition dexpr m l e v := expr m l e (eq v).
+  Definition dexprs m l es vs := list_map (expr m l) es (eq vs).
+
+  Section WithFunctionEnv.
     Context (e: env).
-    Definition dexpr m l e v := expr m l e (eq v).
-    Definition dexprs m l es vs := list_map (expr m l) es (eq vs).
-    (* All cases except cmd.while and cmd.call can be denoted by structural recursion
-       over the syntax.
-       For cmd.while and cmd.call, we fall back to the operational semantics *)
-    Definition cmd_body (rec:_->_->_->_->_->Prop) (c : cmd) (t : trace) (m : mem) (l : locals)
-             (post : trace -> mem -> locals -> Prop) : Prop :=
-      (* give value of each pure expression when stating its subproof *)
-      match c with
-      | cmd.skip => post t m l
-      | cmd.set x ev =>
-        exists v, dexpr m l ev v /\
+    Notation cmd := (Semantics.exec e).
+
+    Definition func '(innames, outnames, c) (t : trace) (m : mem) (args : list word)
+      (post : trace -> mem -> list word -> Prop) :=
+      exists l, map.of_list_zip innames args = Some l /\
+      cmd c t m l (fun t m l =>
+        list_map (get l) outnames (fun rets =>
+        post t m rets)).
+
+    Notation call := Semantics.call (only parsing).
+
+    Definition program := cmd.
+
+    Implicit Type post : trace -> mem -> locals -> Prop.
+
+    Ltac step :=
+      match reverse goal with
+      | H: _ /\ _ |- _ => destruct H
+      | H: exists x, _ |- _ => let n := fresh x in destruct H as [n H]
+      | |- _ => progress unfold dlet, dexpr, store in *
+      | |- _ => constructor
+      | |- _ => assumption
+      | |- _ => progress intros
+      | |- _ => progress subst
+      | H: expr _ _ _ _ |- _ => eapply expr_sound in H
+      | |- _ => solve [econstructor; eauto]
+      end.
+    Ltac tac := repeat step.
+
+    Lemma wp_skip: forall t m l post, post t m l -> cmd cmd.skip t m l post.
+    Proof. tac. Qed.
+
+    Lemma wp_set: forall x ev t m l post,
+        (exists v, dexpr m l ev v /\
         dlet! l := map.put l x v in
-        post t m l
-      | cmd.unset x =>
-        dlet! l := map.remove l x in
-        post t m l
-      | cmd.store sz ea ev =>
-        exists a, dexpr m l ea a /\
+        post t m l) ->
+        cmd (cmd.set x ev) t m l post.
+    Proof. tac. Qed.
+
+    Lemma wp_unset: forall x t m l post,
+        (dlet! l := map.remove l x in
+         post t m l) ->
+        cmd (cmd.unset x) t m l post.
+    Proof. tac. Qed.
+
+    Lemma wp_store: forall sz ea ev t m l post,
+       (exists a, dexpr m l ea a /\
         exists v, dexpr m l ev v /\
         store sz m a v (fun m =>
-        post t m l)
-      | cmd.stackalloc x n c =>
-        Z.modulo n (bytes_per_word width) = 0 /\
+        post t m l)) ->
+       cmd (cmd.store sz ea ev) t m l post.
+    Proof. tac. Qed.
+
+    Lemma wp_stackalloc: forall x n c t m l post,
+        (Z.modulo n (bytes_per_word width) = 0 /\
         forall a mStack mCombined,
           anybytes a n mStack -> map.split mCombined m mStack ->
           dlet! l := map.put l x a in
-          rec c t mCombined l (fun t' mCombined' l' =>
+          cmd c t mCombined l (fun t' mCombined' l' =>
           exists m' mStack',
           anybytes a n mStack' /\ map.split mCombined' m' mStack' /\
-          post t' m' l')
-      | cmd.cond br ct cf =>
-        exists v, dexpr m l br v /\
-        (word.unsigned v <> 0%Z -> rec ct t m l post) /\
-        (word.unsigned v = 0%Z -> rec cf t m l post)
-      | cmd.seq c1 c2 =>
-        rec c1 t m l (fun t m l => rec c2 t m l post)
-      | cmd.while _ _ => Semantics.exec e c t m l post
-      | cmd.call binds fname arges =>
-        exists args, dexprs m l arges args /\
-        Semantics.call e fname t m args (fun t m rets =>
+          post t' m' l')) ->
+          cmd (cmd.stackalloc x n c) t m l post.
+    Proof. tac. Qed.
+
+    Lemma wp_cond: forall br ct cf t m l post,
+        (exists v, dexpr m l br v /\
+        (word.unsigned v <> 0%Z -> cmd ct t m l post) /\
+        (word.unsigned v = 0%Z -> cmd cf t m l post)) ->
+        cmd (cmd.cond br ct cf) t m l post.
+    Proof.
+      tac. destr.destr (Z.eqb (word.unsigned v0) 0).
+      - specialize H1 with (1 := E). tac.
+      - specialize H0 with (1 := E). tac.
+    Qed.
+
+    Lemma wp_seq: forall c1 c2 t m l post,
+        cmd c1 t m l (fun t m l => cmd c2 t m l post) ->
+        cmd (cmd.seq c1 c2) t m l post.
+    Proof. tac. Qed.
+
+    Lemma wp_call: forall binds fname arges t m l post,
+       (exists args, dexprs m l arges args /\
+        call e fname t m args (fun t m rets =>
           exists l', map.putmany_of_list_zip binds rets l = Some l' /\
-          post t m l')
-      | cmd.interact binds action arges =>
-        exists args, dexprs m l arges args /\
+          post t m l')) ->
+       cmd (cmd.call binds fname arges) t m l post.
+    Proof.
+      tac.
+      unfold dexprs in *.
+      eapply exprs_sound in H. destruct H as (argvs & HEv & ?). subst argvs.
+      unfold call in *. fwd.
+      econstructor; eauto.
+    Qed.
+
+    Lemma wp_interact: forall binds action arges t m l post,
+       (exists args, dexprs m l arges args /\
         exists mKeep mGive, map.split m mKeep mGive /\
         ext_spec t mGive action args (fun mReceive rets =>
           exists l', map.putmany_of_list_zip binds rets l = Some l' /\
           forall m', map.split m' mKeep mReceive ->
-          post (cons ((mGive, action, args), (mReceive, rets)) t) m' l')
-      end.
-    Fixpoint cmd c := cmd_body cmd c.
-  End WithFunctions.
-
-  Definition func call '(innames, outnames, c) (t : trace) (m : mem) (args : list word) (post : trace -> mem -> list word -> Prop) :=
-      exists l, map.of_list_zip innames args = Some l /\
-      cmd call c t m l (fun t m l =>
-        list_map (get l) outnames (fun rets =>
-        post t m rets)).
-
-  Definition program := cmd.
+          post (cons ((mGive, action, args), (mReceive, rets)) t) m' l')) ->
+       cmd (cmd.interact binds action arges) t m l post.
+    Proof.
+      tac.
+      eapply exprs_sound in H. destruct H as (argvs & HEv & ?). subst argvs.
+      tac.
+    Qed.
+  End WithFunctionEnv.
 End WeakestPrecondition.
+
+Notation cmd := Semantics.exec (only parsing).
 Notation call := Semantics.call (only parsing).
 
-Ltac unfold1_cmd e :=
-  lazymatch e with
-    @cmd ?width ?BW ?word ?mem ?locals ?ext_spec ?CA ?c ?t ?m ?l ?post =>
-    let c := eval hnf in c in
-    constr:(@cmd_body width BW word mem locals ext_spec CA
-                      (@cmd width BW word mem locals ext_spec CA) c t m l post)
+Ltac apply_rule_for_command c :=
+  lazymatch c with
+  | cmd.skip => eapply wp_skip
+  | cmd.set ?x ?ev => eapply wp_set
+  | cmd.unset ?x => eapply wp_unset
+  | cmd.store ?sz ?ea ?ev => eapply wp_store
+  | cmd.stackalloc ?x ?n ?c => eapply wp_stackalloc
+  | cmd.cond ?br ?ct ?cf => eapply wp_cond
+  | cmd.seq ?c1 ?c2 => eapply wp_seq
+  | cmd.while ?e ?c => fail "cmd.while is not treated in this tactic"
+  | cmd.call ?binds ?fname ?arges => eapply wp_call
+  | cmd.interact ?binds ?action ?arges => eapply wp_interact
   end.
+
 Ltac unfold1_cmd_goal :=
-  let G := lazymatch goal with |- ?G => G end in
-  let G := unfold1_cmd G in
-  change G.
+  lazymatch goal with
+  | |- cmd _ ?c _ _ _ ?post => let c := eval hnf in c in apply_rule_for_command c
+  end.
 
 Ltac unfold1_expr e :=
   lazymatch e with
